some basic definitions

dfy_model/BitVector.dfy
@@ -1,11 +1,16 @@
+include "NativeTypes.dfy"
+
 module CutomBitVector {
+    import opened NativeTypes
+
     datatype cbv_raw = cbv_raw(
-        vals: seq<bool>,
+        vals: seq<uint2>,
         len: nat
     )
 
     type cbv = t: cbv_raw |
-        |t.vals| == t.len witness cbv_raw([], 0)
+        |t.vals| == t.len && t.len >= 1
+        witness cbv_raw([0], 1)
 
     type cbv384 = t: cbv | 
         t.len == 384
@@ -18,6 +23,20 @@ module CutomBitVector {
         return cbv_raw(v1.vals + v2.vals, v1.len + v2.len);
     }
 
-    // method rshift(v1: bv, )
+    function method to_nat(v: cbv) : nat 
+    {
+        to_nat_aux(v.vals)
+    }
 
+    function method to_nat_aux(vals: seq<uint2>) : nat
+    {
+        if |vals| == 0 then 0
+        else vals[0] + 2 * to_nat_aux(vals[1..])
+    }
+
+    method test() 
+    {
+        var a: cbv := cbv_raw([1, 0, 1, 0, 1], 5);
+        assert to_nat(a) == 21;
+    }
 }
